Arm/Insts/DPSFP/Advanced_simd_two_reg_misc.lean
@@ -142,16 +142,16 @@ def exec_advanced_simd_two_reg_misc
   open Std.BitVec in
   let datasize := if inst.Q == 1#1 then 128 else 64 -- 64 << Uint(inst.Q)
   let esize := 8 <<< inst.size.toNat
-  let container_size := 64 >>> ((BitVec.extract inst.opcode 0 0) ++ inst.U).toNat
+  let container_size := 64 >>> ((extractLsb 0 0 inst.opcode) ++ inst.U).toNat
   if h0 : container_size <= esize then
     write_err (StateError.Illegal s!"Illegal {inst} encountered!") s
   else
     have h1 : esize ∣ container_size := by
       simp only [not_le] at h0
-      exact esize_dvd_container_size inst.size (BitVec.extract inst.opcode 0 0 ++ inst.U) h0
+      exact esize_dvd_container_size inst.size (extractLsb 0 0 inst.opcode ++ inst.U) h0
     have h2 : container_size ∣ datasize := by
       simp_all
-      exact container_size_dvd_datasize (BitVec.extract inst.opcode 0 0 ++ inst.U) inst.Q
+      exact container_size_dvd_datasize (extractLsb 0 0 inst.opcode ++ inst.U) inst.Q
     have h3 : 0 < esize := by 
       simp_all only [Nat.sub_zero, Nat.shiftLeft_eq, not_le, IsUnit.mul_iff, beq_iff_eq]
       rw [mul_pos_iff_of_pos_left]
@@ -188,7 +188,7 @@ partial def Advanced_simd_two_reg_misc_cls.rev64_16.rand : IO (Option (BitVec 32
       Rn := ← BitVec.rand 5,
       Rd := ← BitVec.rand 5 }
   let esize := 8 <<< inst.size.toNat
-  let container_size := 64 >>> ((BitVec.extract inst.opcode 0 0) ++ inst.U).toNat
+  let container_size := 64 >>> ((extractLsb 0 0 inst.opcode) ++ inst.U).toNat
   if container_size <= esize then
     -- Keep generating random instructions until a legal one is encountered.
     Advanced_simd_two_reg_misc_cls.rev64_16.rand
@@ -204,7 +204,7 @@ partial def Advanced_simd_two_reg_misc_cls.rev32.rand : IO (Option (BitVec 32)) 
       Rn := ← BitVec.rand 5,
       Rd := ← BitVec.rand 5 }
   let esize := 8 <<< inst.size.toNat
-  let container_size := 64 >>> ((BitVec.extract inst.opcode 0 0) ++ inst.U).toNat
+  let container_size := 64 >>> ((extractLsb 0 0 inst.opcode) ++ inst.U).toNat
   if container_size <= esize then
     -- Keep generating random instructions until a legal one is encountered.
     Advanced_simd_two_reg_misc_cls.rev32.rand
