Arm/Memory.lean
@@ -39,7 +39,7 @@ def write_mem_bytes (n : Nat) (addr : BitVec 64) (val : BitVec (n * 8)) (s : Arm
   match n with
   | 0 => s
   | n' + 1 =>
-    let byte := BitVec.extract val 7 0
+    let byte := extractLsb 7 0 val
     let s := write_mem addr byte s
     let val_rest := Std.BitVec.zeroExtend (n' * 8) (val >>> 8)
     write_mem_bytes n' (addr + 1#64) val_rest s
